I swear I just blinked the the lattice unaxiomatized on its own. How odd, huh?

OwlLean/OwlLang/Owl.lean
@@ -3,20 +3,22 @@ namespace Owl
 structure Lattice where
   labels : Type
   leq    : labels -> labels -> Bool
+  decidable_eq_labels : DecidableEq labels
   bot    : labels
   bot_proof : forall (l : labels), (leq bot l) = true
   join   : labels -> labels -> labels
   meet   : labels -> labels -> labels
 
-axiom L : Lattice
+instance (L : Lattice) : DecidableEq L.labels := L.decidable_eq_labels
 
-abbrev Lcarrier : Type := L.labels
+instance (L : Lattice) : Repr L.labels where
+  reprPrec _ _ := "<lattice label>"
 
 inductive binary : Type
 | bzero : binary -> binary
 | bone : binary -> binary
 | bend : binary
-deriving Repr
+deriving Repr, DecidableEq
 
 inductive cond_sym : Type
 | leq : cond_sym
@@ -27,39 +29,36 @@ inductive cond_sym : Type
 | ngeq : cond_sym
 | ngt : cond_sym
 | nlt : cond_sym
-deriving Repr
+deriving Repr, DecidableEq
 
-instance : Repr Owl.Lcarrier where
-  reprPrec _ _ := "<Lattice Label>"
+inductive label (L : Lattice) : Nat -> Type where
+| var_label : Fin n -> label L n
+| latl : L.labels -> label L n
+| ljoin : label L n -> label L n -> label L n
+| lmeet : label L n -> label L n -> label L n
+| default : label L n
+deriving DecidableEq, Repr
 
-inductive label : Nat -> Type where
-| var_label : Fin n -> label n
-| latl : Lcarrier -> label n
-| ljoin : label n -> label n -> label n
-| lmeet : label n -> label n -> label n
-| default : label n
-deriving Repr
+inductive constr (L : Lattice) (n_label : Nat) : Type where
+| condition : cond_sym -> label L n_label -> label L n_label -> constr L n_label
+deriving Repr, DecidableEq
 
-inductive constr (n_label : Nat) : Type where
-| condition : cond_sym -> label n_label -> label n_label -> constr n_label
-deriving Repr
-
-inductive ty : Nat -> Nat-> Type where
-| var_ty : Fin n_ty -> ty n_label n_ty
-| Any : ty n_label n_ty
-| Unit : ty n_label n_ty
-| Data : label n_label -> ty n_label n_ty
-| Ref : ty n_label n_ty -> ty n_label n_ty
-| arr : ty n_label n_ty -> ty n_label n_ty -> ty n_label n_ty
-| prod : ty n_label n_ty -> ty n_label n_ty -> ty n_label n_ty
-| sum : ty n_label n_ty -> ty n_label n_ty -> ty n_label n_ty
-| all : ty n_label n_ty -> ty n_label (n_ty + 1) -> ty n_label n_ty
-| ex : ty n_label n_ty -> ty n_label (n_ty + 1) -> ty n_label n_ty
-| all_l : cond_sym -> label n_label -> ty (n_label + 1) n_ty -> ty n_label n_ty
-| t_if : constr n_label -> ty n_label n_ty -> ty n_label n_ty -> ty n_label n_ty
-| Public : ty n_label n_ty
-| default : ty n_label n_ty
-deriving Repr
+inductive ty (L : Lattice) : Nat -> Nat-> Type where
+| var_ty : Fin n_ty -> ty L n_label n_ty
+| Any : ty L n_label n_ty
+| Unit : ty L n_label n_ty
+| Data : label L n_label -> ty L n_label n_ty
+| Ref : ty L n_label n_ty -> ty L n_label n_ty
+| arr : ty L n_label n_ty -> ty L n_label n_ty -> ty L n_label n_ty
+| prod : ty L n_label n_ty -> ty L n_label n_ty -> ty L n_label n_ty
+| sum : ty L n_label n_ty -> ty L n_label n_ty -> ty L n_label n_ty
+| all : ty L n_label n_ty -> ty L n_label (n_ty + 1) -> ty L n_label n_ty
+| ex : ty L n_label n_ty -> ty L n_label (n_ty + 1) -> ty L n_label n_ty
+| all_l : cond_sym -> label L n_label -> ty L (n_label + 1) n_ty -> ty L n_label n_ty
+| t_if : constr L n_label -> ty L n_label n_ty -> ty L n_label n_ty -> ty L n_label n_ty
+| Public : ty L n_label n_ty
+| default : ty L n_label n_ty
+deriving Repr, DecidableEq
 
 inductive Dist (a : Type) : Type where
 | ret  : a -> Dist a
@@ -70,46 +69,48 @@ abbrev op := binary -> binary -> Dist binary
 instance : Repr Owl.op where
   reprPrec _ _ := "<Operation>"
 
-inductive tm : Nat -> Nat -> Nat -> Type where
-| var_tm : Fin n_tm -> tm n_label n_ty n_tm
-| error : tm n_label n_ty n_tm
-| skip : tm n_label n_ty n_tm
-| bitstring : binary -> tm n_label n_ty n_tm
-| loc : Nat -> tm n_label n_ty n_tm
-| fixlam : tm n_label n_ty ((n_tm + 1) + 1) -> tm n_label n_ty n_tm
-| tlam : tm n_label (n_ty + 1) n_tm -> tm n_label n_ty n_tm
-| l_lam : tm (n_label + 1) n_ty n_tm -> tm n_label n_ty n_tm
-| Op : op -> tm n_label n_ty n_tm -> tm n_label n_ty n_tm -> tm n_label n_ty n_tm
-| zero : tm n_label n_ty n_tm -> tm n_label n_ty n_tm
-| app : tm n_label n_ty n_tm -> tm n_label n_ty n_tm -> tm n_label n_ty n_tm
-| alloc : tm n_label n_ty n_tm -> tm n_label n_ty n_tm
-| dealloc : tm n_label n_ty n_tm -> tm n_label n_ty n_tm
-| assign : tm n_label n_ty n_tm -> tm n_label n_ty n_tm -> tm n_label n_ty n_tm
-| tm_pair : tm n_label n_ty n_tm -> tm n_label n_ty n_tm -> tm n_label n_ty n_tm
-| left_tm : tm n_label n_ty n_tm -> tm n_label n_ty n_tm
-| right_tm : tm n_label n_ty n_tm -> tm n_label n_ty n_tm
-| inl : tm n_label n_ty n_tm -> tm n_label n_ty n_tm
-| inr {n_label n_ty n_tm} : tm n_label n_ty n_tm -> tm n_label n_ty n_tm
+inductive tm (L : Lattice) : Nat -> Nat -> Nat -> Type where
+| var_tm : Fin n_tm -> tm L n_label n_ty n_tm
+| error : tm L n_label n_ty n_tm
+| skip : tm L n_label n_ty n_tm
+| bitstring : binary -> tm L n_label n_ty n_tm
+| loc : Nat -> tm L n_label n_ty n_tm
+| fixlam : tm L n_label n_ty ((n_tm + 1) + 1) -> tm L n_label n_ty n_tm
+| tlam : tm L n_label (n_ty + 1) n_tm -> tm L n_label n_ty n_tm
+| l_lam : tm L (n_label + 1) n_ty n_tm -> tm L n_label n_ty n_tm
+| Op : op -> tm L n_label n_ty n_tm -> tm L n_label n_ty n_tm -> tm L n_label n_ty n_tm
+| zero : tm L n_label n_ty n_tm -> tm L n_label n_ty n_tm
+| app : tm L n_label n_ty n_tm -> tm L n_label n_ty n_tm -> tm L n_label n_ty n_tm
+| alloc : tm L n_label n_ty n_tm -> tm L n_label n_ty n_tm
+| dealloc : tm L n_label n_ty n_tm -> tm L n_label n_ty n_tm
+| assign : tm L n_label n_ty n_tm -> tm L n_label n_ty n_tm -> tm L n_label n_ty n_tm
+| tm_pair : tm L n_label n_ty n_tm -> tm L n_label n_ty n_tm -> tm L n_label n_ty n_tm
+| left_tm : tm L n_label n_ty n_tm -> tm L n_label n_ty n_tm
+| right_tm : tm L n_label n_ty n_tm -> tm L n_label n_ty n_tm
+| inl : tm L n_label n_ty n_tm -> tm L n_label n_ty n_tm
+| inr {n_label n_ty n_tm} : tm L n_label n_ty n_tm -> tm L n_label n_ty n_tm
 | case :
-    tm n_label n_ty n_tm ->
-    tm n_label n_ty (n_tm + 1) -> tm n_label n_ty (n_tm + 1) -> tm n_label n_ty n_tm
-| tapp : tm n_label n_ty n_tm -> ty n_label n_ty -> tm n_label n_ty n_tm
-| lapp : tm n_label n_ty n_tm -> label n_label -> tm n_label n_ty n_tm
-| pack : ty n_label n_ty -> tm n_label n_ty n_tm -> tm n_label n_ty n_tm
-| unpack : tm n_label n_ty n_tm -> tm n_label (n_ty + 1) (n_tm + 1) -> tm n_label n_ty n_tm
+    tm L n_label n_ty n_tm ->
+    tm L n_label n_ty (n_tm + 1) -> tm L n_label n_ty (n_tm + 1) -> tm L n_label n_ty n_tm
+| tapp : tm L n_label n_ty n_tm -> ty L n_label n_ty -> tm L n_label n_ty n_tm
+| lapp : tm L n_label n_ty n_tm -> label L n_label -> tm L n_label n_ty n_tm
+| pack : ty L n_label n_ty -> tm L n_label n_ty n_tm -> tm L n_label n_ty n_tm
+| unpack : tm L n_label n_ty n_tm -> tm L n_label (n_ty + 1) (n_tm + 1) -> tm L n_label n_ty n_tm
 | if_tm :
-    tm n_label n_ty n_tm ->
-    tm n_label n_ty n_tm -> tm n_label n_ty n_tm -> tm n_label n_ty n_tm
+    tm L n_label n_ty n_tm ->
+    tm L n_label n_ty n_tm -> tm L n_label n_ty n_tm -> tm L n_label n_ty n_tm
 | if_c :
-    constr n_label -> tm n_label n_ty n_tm -> tm n_label n_ty n_tm -> tm n_label n_ty n_tm
-| sync : tm n_label n_ty n_tm -> tm n_label n_ty n_tm
-| annot : tm n_label n_ty n_tm -> ty n_label n_ty -> tm n_label n_ty n_tm
-| default : tm n_label n_ty n_tm
+    constr L n_label -> tm L n_label n_ty n_tm -> tm L n_label n_ty n_tm -> tm L n_label n_ty n_tm
+| sync : tm L n_label n_ty n_tm -> tm L n_label n_ty n_tm
+| annot : tm L n_label n_ty n_tm -> ty L n_label n_ty -> tm L n_label n_ty n_tm
+| default : tm L n_label n_ty n_tm
 deriving Repr
 
+axiom L' : Lattice
+
 -- sanity checks
-#check (tm.error : tm 0 0 0)
-#check (ty.Any : ty 0 0)
+#check (tm.error : tm L' 0 0 0)
+#check (ty.Any : ty L' 0 0)
 
 def ren (m n : Nat) : Type := Fin m → Fin n
 
@@ -147,7 +148,7 @@ def upRen_label_ty (xi : Fin m -> Fin n) : Fin m -> Fin n :=
 
 def ren_label
   (xi_label : Fin m_label → Fin n_label)
-  (s : label m_label) : label n_label :=
+  (s : label L m_label) : label L n_label :=
   match s with
   | .var_label s0 => label.var_label (xi_label s0)
   | .latl s0 => label.latl s0
@@ -156,14 +157,14 @@ def ren_label
   | .default => .default
 
 def ren_constr
-  (xi_label : Fin m_label -> Fin n_label) (s : constr m_label) :
-  constr n_label :=
+  (xi_label : Fin m_label -> Fin n_label) (s : constr L m_label) :
+  constr L n_label :=
   match s with
   | .condition s0 s1 s2 => .condition s0 (ren_label xi_label s1) (ren_label xi_label s2)
 
 def ren_ty
 (xi_label : Fin m_label -> Fin n_label) (xi_ty : Fin m_ty -> Fin n_ty)
-(s : ty m_label m_ty) : ty n_label n_ty :=
+(s : ty L m_label m_ty) : ty L n_label n_ty :=
   match s with
   | .var_ty s0 => .var_ty (xi_ty s0)
   | .Any => .Any
@@ -211,8 +212,8 @@ def upRen_label_tm (xi : Fin m -> Fin n) :
 
 def ren_tm
 (xi_label : Fin m_label -> Fin n_label) (xi_ty : Fin m_ty -> Fin n_ty)
-(xi_tm : Fin m_tm -> Fin n_tm) (s : tm m_label m_ty m_tm) :
-tm n_label n_ty n_tm :=
+(xi_tm : Fin m_tm -> Fin n_tm) (s : tm L m_label m_ty m_tm) :
+tm L n_label n_ty n_tm :=
   match s with
   | .var_tm s0 => .var_tm (xi_tm s0)
   | .error => .error
@@ -283,8 +284,8 @@ tm n_label n_ty n_tm :=
   | .default => .default
 
 def subst_label
-(sigma_label : Fin m_label -> label n_label) (s : label m_label) :
-label n_label :=
+(sigma_label : Fin m_label -> label L n_label) (s : label L m_label) :
+label L n_label :=
   match s with
   | .var_label s0 => sigma_label s0
   | .latl s0 => .latl s0
@@ -295,35 +296,35 @@ label n_label :=
   | .default => .default
 
 def subst_constr
-  (sigma_label : Fin m_label -> label n_label) (s : constr m_label) :
-  constr n_label :=
+  (sigma_label : Fin m_label -> label L n_label) (s : constr L m_label) :
+  constr L n_label :=
   match s with
   | .condition s0 s1 s2 =>
       .condition s0 (subst_label sigma_label s1)
         (subst_label sigma_label s2)
 
-def up_ty_label (sigma : Fin m -> label n_label)
-  : Fin m -> label n_label :=
+def up_ty_label (sigma : Fin m -> label L n_label)
+  : Fin m -> label L n_label :=
     (funcomp (ren_label id) sigma)
 
 def up_ty_ty
-  (sigma : Fin m -> ty n_label n_ty) : Fin (m + 1) -> ty n_label (n_ty + 1) :=
+  (sigma : Fin m -> ty L n_label n_ty) : Fin (m + 1) -> ty L n_label (n_ty + 1) :=
     (cons (.var_ty var_zero)
          (funcomp (ren_ty id shift) sigma))
 
 def up_label_label
-  (sigma : Fin m -> label n_label) : Fin (m + 1) -> label (n_label + 1) :=
+  (sigma : Fin m -> label L n_label) : Fin (m + 1) -> label L (n_label + 1) :=
     (cons (.var_label var_zero)
          (funcomp (ren_label shift) sigma))
 
 def up_label_ty
-  (sigma : Fin m -> ty n_label n_ty) : Fin m -> ty (n_label + 1) n_ty :=
+  (sigma : Fin m -> ty L n_label n_ty) : Fin m -> ty L (n_label + 1) n_ty :=
     (funcomp (ren_ty shift id) sigma)
 
 def subst_ty
-(sigma_label : Fin m_label -> label n_label)
-(sigma_ty : Fin m_ty -> ty n_label n_ty) (s : ty m_label m_ty) :
-ty n_label n_ty :=
+(sigma_label : Fin m_label -> label L n_label)
+(sigma_ty : Fin m_ty -> ty L n_label n_ty) (s : ty L m_label m_ty) :
+ty L n_label n_ty :=
   match s with
   | .var_ty s0 => sigma_ty s0
   | .Any => .Any
